% Einstein求和约定

\section{Einstein求和约定}%
\begin{equation*}
	\begin{aligned}
		& \varepsilon_{ijk}(\partial_i \partial_j \phi)(\partial_k) \\
		&= 
		\frac{1}{2}\varepsilon_{ijk}(\partial_i \partial_j \phi)(\partial_k)
		+
		\frac{1}{2}\varepsilon_{ijk}(\partial_i \partial_j \phi)(\partial_k) \\
		&= 
		\frac{1}{2}\varepsilon_{ijk}(\partial_i \partial_j \phi)(\partial_k) 
		+
		\frac{1}{2}\varepsilon_{jik}(\partial_j \partial_i \phi)(\partial_k) \\
		&= 
		\frac{1}{2}\varepsilon_{ijk}(\partial_i \partial_j \phi)(\partial_k) 
		+
		\frac{1}{2}\varepsilon_{jik}(\partial_i \partial_j \phi)(\partial_k) \\
		&= 
		\frac{1}{2}\varepsilon_{ijk}(\partial_i \partial_j \phi)(\partial_k) 
		-
		\frac{1}{2}\varepsilon_{ijk}(\partial_i \partial_j \phi)(\partial_k)
	\end{aligned}
	\left( kjkj \right)
\end{equation*}





%%% vim: set ts=2 sts=2 sw=2 isk+=\: et cc=+1 formatoptions+=mM:
