% Proof_of_Heisenbergs_Uncertainty_Principle

\section{Proof of Heisenberg's Uncertainty Principle}

Introducing a real coefficient \(\xi\) and an operator \(\hat{F}\), where
\begin{equation}
  -\infty < \xi < \infty
\end{equation}
and
\begin{equation}
  \hat{F} = \xi \hat{A} + i \hat{B} \quad  \hat{F} = \xi \hat{A} - i \hat{B},
\end{equation}
so that
\begin{equation}
  \begin{aligned}
    \hat{F}^\dagger  \hat{F} &= \xi^2 \hat{A}^2 + \hat{B}^2 + i \xi (\hat{A} \hat{B} - \hat{B} \hat{A}) \\
                             &= \xi^2 \hat{A} + \hat{B}^2 - \xi \hat{C}.
  \end{aligned}
\end{equation}
Let
\begin{equation}
  I(\xi) = \Braket{ \hat{F}^\dagger \hat{F} }  = \int \psi^* \hat{F}^\dagger \hat{F} \dd{\tau} = \xi^2 \bar{A}^2 + \bar{B}^2 - \xi \bar{C} \geq 0,
\end{equation}
where
\begin{equation}
  \int \psi^* \hat{F}^\dagger \hat{F} \dd{\tau} = \int \hat{F} \psi ( F \psi )^* \dd{\tau}.
\end{equation}
\begin{equation}
  \implies \bar{A}^2 \bar{B}^2 \geq  \frac{\bar{C}^2}{4}
\end{equation}
\begin{align}
  \hat{A} \rightarrow \hat{A} - \bar{A} \\
  \hat{B} \rightarrow \hat{B} - \bar{B}
\end{align}
\begin{equation}
  \implies \Delta A \cdot \Delta B \geq \frac{\abs{\bar{C}}}{2}
\end{equation}
\begin{equation}
  \Delta x \Delta p_x \geq \frac{\hbar}{2}
\end{equation}



%%% vim: set ts=2 sts=2 sw=2 isk+=\: et cc=+1 formatoptions+=mM:
